ntor/NTOR.ec
@@ -13,17 +13,12 @@ type key_mac, key, tag.
 op [lossless] dtag : tag distr.
 op [lossless] dkey : key distr.
 
-type pr_st_client = s_id * pkey * skey.
-type pr_st_server = s_id * skey * skey option.
-
 clone import GAKE as GAKEc with
   type s_id <- s_id,
   type pkey <- pkey,
   type skey <- skey,
   type key <- key,
   type tag <- tag,
-  type pr_st_client <- pr_st_client,
-  type pr_st_server <- pr_st_server,
   op dskey <- dt,
   op dkey <- dkey,
   op dtag <- dtag.
